pulse/lib/steel/pulse/Pulse.Checker.Auto.Prover.fst
@@ -1,0 +1,220 @@
+module Pulse.Checker.Auto.Prover
+open Pulse.Syntax
+open Pulse.Typing
+open Pulse.Checker.Common
+open Pulse.Checker.VPropEquiv
+module T = FStar.Tactics
+module VP = Pulse.Checker.VPropEquiv
+module F = Pulse.Checker.Framing
+
+let vprop_typing g v = tot_typing g v Tm_VProp
+
+let ghost_comp pre post = 
+  C_STGhost Tm_EmpInames { u=u_zero; res=tm_unit; pre; post }
+
+let unit_const = magic()
+let proof_steps_idem
+  : st_term
+  = { term = Tm_Return { ctag=STT_Ghost; insert_eq=false; term=unit_const};
+      range = Range.range_0 }
+let proof_steps_idem_typing (g:env) (ctxt:vprop)
+  : st_typing g proof_steps_idem (ghost_comp ctxt ctxt)
+  = magic()
+
+let comp_st_with_post (c:comp_st) (post:term) : c':comp_st { st_comp_of_comp c' == ({ st_comp_of_comp c with post} <: st_comp) } =
+  match c with
+  | C_ST st -> C_ST { st with post }
+  | C_STGhost i st -> C_STGhost i { st with post }
+  | C_STAtomic i st -> C_STAtomic i {st with post}
+
+let comp_st_with_pre (c:comp_st) (pre:term) : comp_st =
+  match c with
+  | C_ST st -> C_ST { st with pre }
+  | C_STGhost i st -> C_STGhost i { st with pre }
+  | C_STAtomic i st -> C_STAtomic i {st with pre }
+
+assume
+val post_with_emp (#g:env) (#t:st_term) (#c:comp_st) (d:st_typing g t c)
+  : st_typing g t (comp_st_with_post c (Tm_Star (canon_vprop (comp_post c)) Tm_Emp) )
+
+module Metatheory = Pulse.Typing.Metatheory
+
+let vprop_equiv_x g t p1 p2 =
+  x:var { Metatheory.fresh_wrt x g (freevars p1) } ->
+  vprop_equiv (extend x (Inl t) g) 
+              (open_term p1 x)
+              (open_term p2 x)
+
+assume
+val st_typing_equiv_post (#g:env) (#t:st_term) (#c:comp_st) (d:st_typing g t c)
+                         (#post:term )//{ freevars post `Set.subset` freevars (comp_post c)}
+                         (veq: vprop_equiv_x g (comp_res c) (comp_post c) post)
+  : st_typing g t (comp_st_with_post c post)
+
+assume
+val st_typing_equiv_pre (#g:env) (#t:st_term) (#c:comp_st) (d:st_typing g t c)
+                        (#pre:term )//{ freevars post `Set.subset` freevars (comp_post c)}
+                        (veq: vprop_equiv g (comp_pre c) pre)
+  : st_typing g t (comp_st_with_pre c pre)
+
+
+noeq
+type prover_state (g:env) (ctxt:vprop) = {
+  (* the original context is well-typed *)
+  ctxt_typing: vprop_typing g ctxt;
+  (* the program whose precondition we're trying to derive *)
+  t:st_term;
+  c:comp_st;
+  t_typing:st_typing g t c;
+  (* the in-progress proof state *)
+  matched_pre:term; (* conjuncts that we have already derived *)
+  unmatched_pre:list term; (* conjuncts remaining to be derived *)
+  remaining_ctxt:list term; (* unused conjuncts in the context *)
+  (* Ghost proof steps witnessing the derivation of matched_pre from ctxt *)
+  proof_steps: st_term;
+  proof_steps_typing: st_typing g proof_steps (ghost_comp ctxt (Tm_Star (list_as_vprop remaining_ctxt) matched_pre));
+  pre_equiv:vprop_equiv g (comp_pre c) (Tm_Star (list_as_vprop unmatched_pre) matched_pre);
+}
+
+let proof_steps_post #g #o (p:prover_state g o) : vprop = Tm_Star (list_as_vprop p.remaining_ctxt) p.matched_pre
+
+let bind_proof_steps_with #g #o (p:prover_state g o) 
+                                (t:st_term)
+                                (c:comp_st {comp_pre c == proof_steps_post p})
+                                (t_typing:st_typing g t c)
+   : (t':st_term & st_typing g t' (comp_st_with_pre c o))
+   = admit()
+
+let init_prover_state (#g:env) (#ctxt:vprop) (ctxt_typing: vprop_typing g ctxt)
+                      (#t:st_term) (#c:comp_st) (t_typing: st_typing g t c)
+  : prover_state g ctxt
+  = { 
+        ctxt_typing;
+        t; 
+        c; 
+        t_typing;
+
+        matched_pre = Tm_Emp;
+        unmatched_pre = vprop_as_list (comp_pre c);
+        remaining_ctxt = vprop_as_list ctxt;
+
+        pre_equiv = VE_Trans _ _ _ _ (vprop_list_equiv _ (comp_pre c))
+                                     (VE_Sym _ _ _ (VP.ve_unit_r _ (canon_vprop (comp_pre c))));
+        proof_steps=proof_steps_idem;
+        proof_steps_typing=post_with_emp (proof_steps_idem_typing _ ctxt);
+    }
+
+noeq
+type match_result g p ctxt = {
+  matched:list vprop;
+  unmatched:list vprop;
+  ctxt':list vprop;
+  p_eq: vprop_equiv g (list_as_vprop p) (list_as_vprop (unmatched @ matched));
+  ctxt_eq: vprop_equiv g (list_as_vprop ctxt) (list_as_vprop (ctxt' @ matched))
+}
+
+open FStar.List.Tot 
+
+assume
+val all_simple_matches (g:env) (p:list vprop) (ctxt:list vprop)
+  : T.Tac (option (match_result g p ctxt))
+
+let step_t = #g:_ -> #o:_ -> p:prover_state g o -> T.Tac (option (prover_state g o))
+
+let step_match : step_t = 
+  fun #g #o (p:prover_state g o) ->
+    match all_simple_matches g p.unmatched_pre p.remaining_ctxt with
+    | None -> None
+    | Some res ->
+      let matched_pre = Tm_Star (list_as_vprop res.matched) p.matched_pre in
+        // remaining_ctxt ~ res.ctxt' * res.matched
+      let veq 
+        : vprop_equiv_x g tm_unit 
+                          (Tm_Star (list_as_vprop p.remaining_ctxt) p.matched_pre)
+                          (Tm_Star (list_as_vprop res.ctxt') matched_pre)
+        = magic ()
+      in
+        // p.unmatched_pre ~ res.unmatched @ res.matched
+      let pre_equiv
+          : vprop_equiv g (comp_pre p.c) (Tm_Star (list_as_vprop res.unmatched) matched_pre)
+          = magic ()
+      in
+      let proof_steps_typing = st_typing_equiv_post p.proof_steps_typing veq in
+      Some 
+        { p with unmatched_pre = res.unmatched;
+                 matched_pre;
+                 remaining_ctxt = res.ctxt';
+                 proof_steps_typing;
+                 pre_equiv }
+
+let step_intro_exists #g #o (p:prover_state g o) : T.Tac (option (prover_state g o)) = None
+
+let step_intro_pure #g #o (p:prover_state g o) : T.Tac (option (prover_state g o)) = None
+let step_intro_rewrite #g #o (p:prover_state g o) : T.Tac (option (prover_state g o)) = None
+
+let rec first_success (l:list step_t) : step_t = 
+  fun #g #o p ->
+    match l with
+    | [] -> None
+    | s :: l -> 
+      match s p with
+      | None -> first_success l p
+      | Some p -> Some p
+
+(* Take one step of proving, matching at least one unmatched pre, or rewriting the context.
+   If neither, then returns None; and the outer loop should fail reporting unmatched preconditions *)
+let step : step_t
+  = first_success [ step_match <: step_t;
+                    step_intro_exists <: step_t;
+                    step_intro_pure <: step_t;
+                    step_intro_rewrite <: step_t ]
+
+                                //  
+let finish #g #o (p:prover_state g o { p.unmatched_pre == []})
+  : (t:st_term & c:comp_st { comp_pre c == o } & st_typing g t c)
+  = assume (list_as_vprop [] == Tm_Emp);
+    let veq1 : vprop_equiv _ (comp_pre p.c) p.matched_pre = VE_Trans _ _ _ _ p.pre_equiv (VE_Unit _ _) in
+    let t_typing : st_typing g p.t (comp_st_with_pre p.c p.matched_pre) = st_typing_equiv_pre p.t_typing veq1 in
+    let remaining_context_typing : vprop_typing g (list_as_vprop p.remaining_ctxt) = magic () in
+    let framing_token : F.frame_for_req_in_ctxt g (proof_steps_post p) p.matched_pre =
+      (| list_as_vprop p.remaining_ctxt,
+         remaining_context_typing,
+         VE_Comm _ _ _ |)
+    in
+    let ctxt_typing : vprop_typing g (proof_steps_post p) = magic () in
+    let (| _, t_typing |) = F.apply_frame ctxt_typing t_typing framing_token in
+    let (| t, t_typing |) = bind_proof_steps_with p _ _ t_typing in
+    (| _, _, t_typing |)
+
+let as_failure #g #o (p:prover_state g o) = {
+  unmatched_preconditions = p.unmatched_pre;
+  remaining_context = p.remaining_ctxt
+}
+
+let rec solve #g #o (p:prover_state g o)
+  : T.Tac 
+    (either 
+        (t:st_term &
+         c:comp_st { comp_pre c == o } &
+         st_typing g t c)
+        framing_failure)
+  = match step p with
+    | None -> Inr (as_failure p)
+    | Some p ->
+      match p.unmatched_pre with
+      | [] -> Inl (finish p)
+      | _ -> solve p
+
+let prove_precondition (#g:env)
+                       (#ctxt:term)
+                       (ctxt_typing: tot_typing g ctxt Tm_VProp)
+                       (#t:st_term)
+                       (#c:comp_st)
+                       (t_typing: st_typing g t c)
+  : T.Tac 
+    (either 
+        (t:st_term &
+         c:comp_st { comp_pre c == ctxt } &
+         st_typing g t c)
+        framing_failure)
+   = solve (init_prover_state ctxt_typing t_typing)
